CHERI_Fetch_Properties.thy
@@ -1,0 +1,42 @@
+theory CHERI_Fetch_Properties
+  imports CHERI_Mem_Properties
+begin
+
+context Morello_Fetch_Automaton
+begin
+
+lemmas non_cap_exp_traces_enabled[traces_enabledI] = non_cap_expI[THEN non_cap_exp_traces_enabledI]
+
+lemmas non_mem_exp_traces_enabled[traces_enabledI] = non_mem_expI[THEN non_mem_exp_traces_enabledI]
+
+lemma traces_enabled_Mem_read_Fetch[traces_enabledI]:
+  assumes "\<And>v. paccess_enabled s Fetch (unat (FullAddress_address (AddressDescriptor_paddress desc))) (nat sz) v B0"
+  shows "traces_enabled (Mem_read desc sz accdesc) s"
+  unfolding Mem_read_def bind_assoc
+  by (traces_enabledI intro: traces_enabled_read_mem assms: assms)
+
+lemma load_enabled_access_enabled_Fetch[intro]:
+  assumes "load_enabled s acctype vaddr sz tagged"
+    and "sz' = nat sz"
+    and "translate_address vaddr = Some paddr"
+    and "tagged \<or> tag = B0"
+  shows "\<exists>vaddr. access_enabled s Fetch vaddr paddr sz' data tag"
+  using assms
+  unfolding load_enabled_def
+  by (cases tagged) auto
+
+lemma traces_enabled_AArch64_MemSingle_read[traces_enabledI]:
+  assumes "translate_address (unat address) \<noteq> None \<longrightarrow> load_enabled s acctype (unat address) size__arg False"
+  shows "traces_enabled (AArch64_MemSingle_read address size__arg acctype wasaligned :: 'size_times_p8::len word M) s"
+  unfolding AArch64_MemSingle_read_def bind_assoc
+  by (traces_enabledI assms: assms intro: traces_enabled_Mem_read_Fetch simp: exp_fails_if_then_else)
+
+lemma traces_enabled_FetchInstr[traces_enabledI]:
+  assumes "{''PCC''} \<subseteq> accessible_regs s"
+  shows "traces_enabled (FetchInstr pc) s"
+  unfolding FetchInstr_def CheckPCCCapability_def bind_assoc
+  by (traces_enabledI assms: assms elim: CheckCapability_load_enabled intro: derivable_or_invokedI1)
+
+end
+
+end
